src/Serial.v
@@ -2,166 +2,87 @@ Require Import Bool List String Peano_dec.
 Require Import Permutation.
 Require Import Common FMap Syntax Semantics.
 
-(* [sys] as a requester for [msg] *)
-Definition asRequester (sys: System) (msg: Msg) :=
-  if mid_rq (msg_id msg) ?<n (indicesOf sys) then true else false.
+Section PerSystem.
+  Variable sys: System.
+  Variable step: System -> State -> Label -> State -> Prop.
 
-(* [sys] as a responder for [msg] *)
-Definition asResponder (sys: System) (msg: Msg) :=
-  if mid_rs (msg_id msg) ?<n (indicesOf sys) then true else false.
+  Record HLabel :=
+    { hlbl_hdl : Msg;
+      hlbl_outs : list Msg
+    }.
 
-Definition rqSubHistory (sys: System) (hst: list Msg) :=
-  filter (asRequester sys) hst.
-Definition rsSubHistory (sys: System) (hst: list Msg) :=
-  filter (asResponder sys) hst.
+  Definition toHLabel (l: Label): option HLabel :=
+    match l with
+    | {| lbl_hdl := None |} => None
+    | {| lbl_hdl := Some h; lbl_outs := outs |} =>
+      Some {| hlbl_hdl := h; hlbl_outs := outs |}
+    end.
 
-Definition History := list Msg.
+  Definition History := list HLabel.
 
-(* For a given system [sys] and its trace [tr], the history of [tr] is a request
- * subhistory with respect to [sys], where [lbl_hdl] is ignored.
- *)
-Fixpoint historyOf (sys: System) (tr: list BLabel): History :=
-  match tr with
-  | nil => nil
-  | {| blbl_ins := ins; blbl_outs := outs |} :: tr' =>
-    (rsSubHistory sys (outs ++ ins)) ++ (historyOf sys tr')
-  end.
+  Fixpoint historyOf (ll: list Label): History :=
+    match ll with
+    | nil => nil
+    | lbl :: ll' => (toHLabel lbl) ::> (historyOf ll')
+    end.
 
-Inductive HistoryOf (step: System -> State -> Label -> State -> Prop)
-  : System -> History -> Prop :=
-| Hist: forall sys tr,
-    Behavior step sys tr ->
-    HistoryOf step sys (historyOf sys tr).
+  Inductive HistoryOf: History -> Prop :=
+  | Hist: forall ll st,
+      steps step sys (getStateInit sys) ll st ->
+      HistoryOf (historyOf ll).
 
-(* A history consisting only of requests and matching responses. *)
-Inductive Complete: list Msg -> Prop :=
-| CplNil: Complete nil
-| CplAdd:
-    forall hst1 hst2 hst3,
-      Complete (hst1 ++ hst2 ++ hst3) ->
-      forall rq rs,
-        isTrsPair (msg_id rq) (msg_id rs) = true ->
-        forall chst,
-          chst = hst1 ++ rq :: hst2 ++ rs :: hst3 ->
-          Complete chst.
+  Inductive Atomic: Msg -> History -> list Msg -> Prop :=
+  | AtomicBase:
+      forall min hlbl mouts,
+        hlbl = {| hlbl_hdl := min; hlbl_outs := mouts |} ->
+        Atomic min (hlbl :: nil) mouts
+  | AtomicCons:
+      forall min hst mouts,
+        Atomic min hst mouts ->
+        forall hdl houts,
+          In hdl mouts ->
+          Atomic min ({| hlbl_hdl := hdl; hlbl_outs := houts |} :: hst)
+                 (List.remove msg_dec hdl mouts ++ houts).
 
-Inductive SubHistory: list Msg -> list Msg -> Prop :=
-| ShNil: SubHistory nil nil
-| ShAdd: forall l1 l2, SubHistory l1 l2 -> forall a, SubHistory (a :: l1) (a :: l2)
-| ShSkip: forall l1 l2, SubHistory l1 l2 -> forall a, SubHistory l1 (a :: l2).
+  Definition AtomicTrs (hst: History) :=
+    exists min mout,
+      isTrsPair (msg_id min) (msg_id mout) = true /\
+      Atomic min hst (mout :: nil).
 
-Definition ExtHistory {A} (l el: list A): Prop :=
-  exists e, el = l ++ e.
+  Definition IncompleteTrs (hst: History) :=
+    exists min mouts,
+      Forall (fun m => isInternal sys (msgTo (msg_id m)) = true) mouts /\
+      Atomic min hst mouts.
 
-Fixpoint matchTrsPair (rq: Msg) (rss: list Msg) :=
-  match rss with
-  | nil => None
-  | rs :: rss' =>
-    if isTrsPair (msg_id rq) (msg_id rs) then Some rss'
-    else match matchTrsPair rq rss' with
-         | Some nrss => Some (rs :: nrss)
-         | None => None
-         end
-  end.
+  Definition Sequential (hst: History) :=
+    exists (trs: list History),
+      Forall (fun h => AtomicTrs h \/ IncompleteTrs h) trs /\
+      hst = concat trs.
 
-Fixpoint complete' (hst rss: list Msg): list Msg * list Msg :=
-  match hst with
-  | nil => (nil, rss)
-  | msg :: hst' =>
-    match mid_rqrs (msg_id msg) with
-    | Rq => let (phst, prss) := complete' hst' rss in
-            match matchTrsPair msg prss with
-            | Some nrss => (msg :: phst, nrss)
-            | None => (phst, prss)
-            end
-    | Rs => let (phst, prss) := complete' hst' rss in
-            (msg :: phst, msg :: prss)
-    end
-  end.
+End PerSystem.
 
-Definition complete (hst: list Msg) := fst (complete' hst nil).
-Definition WellFormed (hst: list Msg) := snd (complete' hst nil) = nil.
-
-Lemma complete_subList: forall hst, SubHistory (complete hst) hst.
-Proof.
-Admitted.
-
-Lemma complete_complete: forall hst, Complete (complete hst).
-Proof.
-Admitted.
-
-Lemma complete_maximal:
-  forall hst chst,
-    chst <> complete hst ->
-    SubHistory chst hst -> Complete chst ->
-    ~ SubHistory (complete hst) chst.
-Proof.
-Admitted.
-
-(* A history [hst] is [Sequential] if:
- * 1) the first message is a request,
- * 2) a matching response for each request is right after the request, and
- * 3) there might not be a matching response for the last request.
- *)
-Fixpoint Sequential' (hst: list Msg) (orq: option Msg) :=
-  match hst with
-  | nil => true
-  | msg :: hst' =>
-    match orq with
-    | Some rq => isTrsPair (msg_id rq) (msg_id msg) && Sequential' hst' None
-    | None => match mid_rqrs (msg_id msg) with
-              | Rq => Sequential' hst' (Some msg)
-              | Rs => false
-              end
-    end
-  end.
-Definition Sequential (hst: list Msg) := Sequential' hst None = true.
-Definition Concurrent (hst: list Msg) := ~ Sequential hst.
-
-Definition sequential_concurrent_dec:
-  forall hst, {Sequential hst} + {Concurrent hst}.
-Proof.
-  unfold Concurrent, Sequential; intros.
-  destruct (Sequential' hst None).
-  - left; reflexivity.
-  - right; discriminate.
-Defined.
-
-(* A system is sequential when all possible histories are sequential. *)
-Definition SequentialSys (step: System -> State -> Label -> State -> Prop)
-           (sys: System) :=
-  forall hst, HistoryOf step sys hst -> Sequential (rev hst).
-
-Definition requestsOf (hst: list Msg) :=
-  filter (fun m => match mid_rqrs (msg_id m) with
-                   | Rq => true
-                   | _ => false
-                   end) hst.
+Definition insOf (obj: Object) (hst: History) :=
+  filter (fun hl =>
+            if obj_idx obj ==n msgFrom (msg_id (hlbl_hdl hl))
+            then true else false) hst.
 
 (* Two histories are equivalent if
  * 1) one history is a permutation of the other, and
- * 2) they have the same request orders per an object.
+ * 2) they have the same in-orders per an object.
  *)
-Definition Equivalent (hst1 hst2: list Msg) :=
+Definition Equivalent (hst1 hst2: History) :=
   Permutation hst1 hst2 /\
-  forall obj, requestsOf (rqSubHistory [obj] hst1) =
-              requestsOf (rqSubHistory [obj] hst2).
+  forall obj, insOf obj hst1 = insOf obj hst2.
 
-(* NOTE: this may not be a complete definition:
- * Strict serializability (in concurrent system) requires one more condition: 
- * any _strict_ transaction orders are preserved by the serial history [shst].
- * I'm currently not sure if we need the second condition for message-passing 
- * systems.
- *)
-Definition Serializable (hst shst: list Msg) :=
-  Sequential shst /\
-  Equivalent (complete hst) shst.
+Infix "≡" := Equivalent (at level 30).
+
+Definition Serializable (sys: System) (hst shst: History) :=
+  Sequential sys shst /\ Equivalent hst shst.
 
 (* A system is [Serial] when all possible histories are [Serializable]. *)
-Definition Serial (step: System -> State -> Label -> State -> Prop)
-           (sys: System) :=
+Definition Serial (sys: System) (step: System -> State -> Label -> State -> Prop) :=
   forall hst,
-    HistoryOf step sys hst ->
-    exists lhst, HistoryOf step sys lhst /\
-                 Serializable (rev hst) (rev lhst).
+    HistoryOf sys step hst ->
+    exists shst, HistoryOf sys step shst /\
+                 Serializable sys hst shst.
 
