src/SerialFacts.v
@@ -2,10 +2,28 @@ Require Import Bool List String Peano_dec.
 Require Import Permutation.
 Require Import Common FMap Syntax Semantics SemDet SemSeq Serial.
 
+Set Implicit Arguments.
+
+Lemma steps_history:
+  forall sys step tr st,
+    steps step sys (getStateInit sys) tr st ->
+    HistoryOf sys step (historyOf tr).
+Proof.
+  intros.
+  econstructor; eauto.
+Qed.
+
 Theorem sequential_step_seq:
   forall sys,
-    Serial step_det sys ->
-    step_det # step_seq |-- sys ⊑[id] sys.
+    Serial sys step_mod -> step_mod # step_seq |-- sys ⊑[id] sys.
 Proof.
+  unfold Serial, Refines; intros.
+  rewrite map_id.
+  inv H0; rename ll0 into ill. (* ill: the interleaving label sequence *)
+  pose proof (steps_history H1); clear H1 st.
+  specialize (H _ H0); destruct H as [shst [? ?]]; clear H0.
+
+  inv H.
+  inv H1.
 Admitted.
 
